\subsection{} % 4.3
    Rearrange:
    \begin{align*}
        &ğ•ƒ_{n}\left(\sqrt{n^{2}+1}+\left(n+1\right)^{2}-an^{2}-bn\right) \\
        =&ğ•ƒ_{n}\left(\sqrt{n^{2}+1}+\left(n+1\right)+n\left(n+1\right)-an^{2}-bn\right) \\
        =&ğ•ƒ_{n}\left(\sqrt{n^{2}+1}+\left(1-a\right)n^{2}+\left(2-b\right)n+1\right) \\
        =&ğ•ƒ_{n}\left(\sqrt{n^{2}+1}+\left(1-a\right)n^{2}+\left(2-b\right)n\right)+1 \\
        =&ğ•ƒ_{n}\left(\sqrt{n^{2}+1}+\left(1-a\right)n^{2}+\left(2-b\right)n\right)+1
    \end{align*}
    
    Let $a=1$ and $b=3$
    \begin{align*}
        &ğ•ƒ_{n}\left(\sqrt{n^{2}-1}-n\right) \\
        =&ğ•ƒ_{n}\left(\left(\sqrt{n^{2}-1}-n\right)\frac{\left(\sqrt{n^{2}-1}+n\right)}{\left(\sqrt{n^{2}-1}+n\right)}\right) \\
        =&ğ•ƒ_{n}\left(-\frac{1}{\sqrt{n^{2}-1}+n}\right) \\
        &ğ•¥{Use the fact that} \sqrt{n^{2}-1}+n\ \ge\ n \\
        =&0
    \end{align*}
    $$ğ•¥{Bring back the 1 from earlier}$$
    $$ğ•ƒ_{n}\left(\sqrt{n^{2}+1}+\left(n+1\right)^{2}-an^{2}-bn\right)=1$$ \qed